generic/Zeta.Generic.Thread.fsti
@@ -108,6 +108,11 @@ let is_within_epoch #vspec (ep: epoch)
 
 open Zeta.AppSimulate
 
+let is_appfn_within_epoch #vspec (ep: epoch)
+  (tl: verifiable_log vspec) (i: seq_index tl)
+  = is_appfn tl i &&
+    is_within_epoch ep tl i
+
 (* for an appfn entry, return the function call params and result *)
-val appfn_call_res (#vspec:_) (ep: epoch):
-  cond_idxfn_t #vspec (appfn_call_res vspec.app) (conj is_appfn (is_within_epoch ep))
+val to_appfn_call_res (#vspec:_) (ep: epoch):
+  cond_idxfn_t #vspec (appfn_call_res vspec.app) (is_appfn_within_epoch ep)
