high2/Zeta.High.Interleave.fsti
@@ -1,0 +1,8 @@
+module Zeta.High.Interleave
+
+open Zeta.App
+open Zeta.Generic.Interleave
+open Zeta.High.Verifier
+
+let ilog (app: app_params) = Zeta.Generic.Interleave.ilog (high_verifier_spec app)
+
